hax-lib/proof-libs/fstar/core/Alloc.Collections.Binary_heap.fst
@@ -9,12 +9,58 @@ type t_BinaryHeap (v_T: Type0) (v_A: Type0) =
   | BinaryHeap : Alloc.Vec.t_Vec v_T Alloc.Alloc.t_Global -> Core_models.Marker.t_PhantomData v_A
     -> t_BinaryHeap v_T v_A
 
-let impl_10__new
-      (#v_T: Type0)
-      (#v_A: Type0)
-      (#[FStar.Tactics.Typeclasses.tcresolve ()] i0: Core_models.Cmp.t_Ord v_T)
-      (#[FStar.Tactics.Typeclasses.tcresolve ()] i1: Alloc.Alloc.t_Allocator v_A)
-      (_: Prims.unit)
+/// See [`std::collections::binary_heap::Iter`]
+type t_Iter (v_T: Type0) = | Iter : Rust_primitives.Sequence.t_Seq v_T -> t_Iter v_T
+
+[@@ FStar.Tactics.Typeclasses.tcinstance]
+let impl (#v_T: Type0) : Core_models.Iter.Traits.Iterator.t_Iterator (t_Iter v_T) =
+  {
+    f_Item = v_T;
+    f_next_pre = (fun (self: t_Iter v_T) -> true);
+    f_next_post
+    =
+    (fun (self: t_Iter v_T) (out1: (t_Iter v_T & Core_models.Option.t_Option v_T)) -> true);
+    f_next
+    =
+    fun (self: t_Iter v_T) ->
+      let (self: t_Iter v_T), (hax_temp_output: Core_models.Option.t_Option v_T) =
+        if (Rust_primitives.Sequence.seq_len #v_T self._0 <: usize) =. mk_usize 0
+        then
+          self, (Core_models.Option.Option_None <: Core_models.Option.t_Option v_T)
+          <:
+          (t_Iter v_T & Core_models.Option.t_Option v_T)
+        else
+          let (tmp0: Rust_primitives.Sequence.t_Seq v_T), (out: v_T) =
+            Rust_primitives.Sequence.seq_remove #v_T self._0 (mk_usize 0)
+          in
+          let self:t_Iter v_T = { self with _0 = tmp0 } <: t_Iter v_T in
+          self, (Core_models.Option.Option_Some out <: Core_models.Option.t_Option v_T)
+          <:
+          (t_Iter v_T & Core_models.Option.t_Option v_T)
+      in
+      self, hax_temp_output <: (t_Iter v_T & Core_models.Option.t_Option v_T)
+  }
+
+/// See [`std::collections::BinaryHeap::new`]
+let impl_9__new (#v_T: Type0) (_: Prims.unit) : t_BinaryHeap v_T Alloc.Alloc.t_Global =
+  BinaryHeap
+    (Alloc.Vec.from_seq #v_T
+        #Alloc.Alloc.t_Global
+        (Rust_primitives.Sequence.seq_empty #v_T () <: Rust_primitives.Sequence.t_Seq v_T))
+    (Core_models.Marker.PhantomData <: Core_models.Marker.t_PhantomData Alloc.Alloc.t_Global)
+  <:
+  t_BinaryHeap v_T Alloc.Alloc.t_Global
+
+/// See [`std::collections::BinaryHeap::with_capacity`]: capacity is
+/// not modeled, so this is `new`.
+let impl_9__with_capacity (#v_T: Type0) (e_capacity: usize) : t_BinaryHeap v_T Alloc.Alloc.t_Global =
+  impl_9__new #v_T ()
+
+/// See [`std::collections::BinaryHeap::new_in`]
+let impl_10__new_in
+      (#v_T #v_A: Type0)
+      (#[FStar.Tactics.Typeclasses.tcresolve ()] i0: Alloc.Alloc.t_Allocator v_A)
+      (e_alloc: v_A)
     : t_BinaryHeap v_T v_A =
   BinaryHeap
     (Alloc.Vec.from_seq #v_T
@@ -24,17 +70,71 @@ let impl_10__new
   <:
   t_BinaryHeap v_T v_A
 
+/// See [`std::collections::BinaryHeap::with_capacity_in`]
+let impl_10__with_capacity_in
+      (#v_T #v_A: Type0)
+      (#[FStar.Tactics.Typeclasses.tcresolve ()] i0: Alloc.Alloc.t_Allocator v_A)
+      (e_capacity: usize)
+      (alloc: v_A)
+    : t_BinaryHeap v_T v_A = impl_10__new_in #v_T #v_A alloc
+
+/// See [`std::collections::BinaryHeap::retain`].
+/// DEVIATION(std): bounded by `Fn`, not `FnMut` — see the note on
+/// `vec_deque`. The loop walks from the back so a removal never
+/// shifts an index still to be visited.
+/// Opaque for F* only, like `VecDeque::retain`: hax does not emit
+/// the `f_Output == bool` constraint for a `Fn` bound.
+assume
+val impl_10__retain':
+    #v_T: Type0 ->
+    #v_A: Type0 ->
+    #v_F: Type0 ->
+    {| i0: Alloc.Alloc.t_Allocator v_A |} ->
+    {| i1: Core_models.Ops.Function.t_Fn v_F v_T |} ->
+    {| i2: Core_models.Cmp.t_Ord v_T |} ->
+    self: t_BinaryHeap v_T v_A ->
+    f: v_F
+  -> t_BinaryHeap v_T v_A
+
+unfold
+let impl_10__retain
+      (#v_T #v_A #v_F: Type0)
+      (#[FStar.Tactics.Typeclasses.tcresolve ()] i0: Alloc.Alloc.t_Allocator v_A)
+      (#[FStar.Tactics.Typeclasses.tcresolve ()] i1: Core_models.Ops.Function.t_Fn v_F v_T)
+      (#[FStar.Tactics.Typeclasses.tcresolve ()] i2: Core_models.Cmp.t_Ord v_T)
+     = impl_10__retain' #v_T #v_A #v_F #i0 #i1 #i2
+
+/// See [`std::collections::BinaryHeap::into_sorted_vec`]: ascending.
+/// Opaque: the Rust body below is the specification (repeatedly move
+/// out the smallest remaining element), but proving the `Vec::push`
+/// bound through the loop needs an invariant relating two locals,
+/// which `hax_lib::loop_invariant!` cannot state here.
+assume
+val impl_10__into_sorted_vec':
+    #v_T: Type0 ->
+    #v_A: Type0 ->
+    {| i0: Alloc.Alloc.t_Allocator v_A |} ->
+    {| i1: Core_models.Cmp.t_Ord v_T |} ->
+    self: t_BinaryHeap v_T v_A
+  -> Alloc.Vec.t_Vec v_T Alloc.Alloc.t_Global
+
+unfold
+let impl_10__into_sorted_vec
+      (#v_T #v_A: Type0)
+      (#[FStar.Tactics.Typeclasses.tcresolve ()] i0: Alloc.Alloc.t_Allocator v_A)
+      (#[FStar.Tactics.Typeclasses.tcresolve ()] i1: Core_models.Cmp.t_Ord v_T)
+     = impl_10__into_sorted_vec' #v_T #v_A #i0 #i1
+
 let impl_11__len
       (#v_T #v_A: Type0)
-      (#[FStar.Tactics.Typeclasses.tcresolve ()] i0: Core_models.Cmp.t_Ord v_T)
-      (#[FStar.Tactics.Typeclasses.tcresolve ()] i1: Alloc.Alloc.t_Allocator v_A)
+      (#[FStar.Tactics.Typeclasses.tcresolve ()] i0: Alloc.Alloc.t_Allocator v_A)
       (self: t_BinaryHeap v_T v_A)
     : usize = Alloc.Vec.impl_1__len #v_T #Alloc.Alloc.t_Global self._0
 
 let impl_10__push
       (#v_T #v_A: Type0)
-      (#[FStar.Tactics.Typeclasses.tcresolve ()] i0: Core_models.Cmp.t_Ord v_T)
-      (#[FStar.Tactics.Typeclasses.tcresolve ()] i1: Alloc.Alloc.t_Allocator v_A)
+      (#[FStar.Tactics.Typeclasses.tcresolve ()] i0: Alloc.Alloc.t_Allocator v_A)
+      (#[FStar.Tactics.Typeclasses.tcresolve ()] i1: Core_models.Cmp.t_Ord v_T)
       (self: t_BinaryHeap v_T v_A)
       (v: v_T)
     : Prims.Pure (t_BinaryHeap v_T v_A)
@@ -49,8 +149,8 @@ let impl_10__push
 
 let impl_10__pop
       (#v_T #v_A: Type0)
-      (#[FStar.Tactics.Typeclasses.tcresolve ()] i0: Core_models.Cmp.t_Ord v_T)
-      (#[FStar.Tactics.Typeclasses.tcresolve ()] i1: Alloc.Alloc.t_Allocator v_A)
+      (#[FStar.Tactics.Typeclasses.tcresolve ()] i0: Alloc.Alloc.t_Allocator v_A)
+      (#[FStar.Tactics.Typeclasses.tcresolve ()] i1: Core_models.Cmp.t_Ord v_T)
       (self: t_BinaryHeap v_T v_A)
     : Prims.Pure (t_BinaryHeap v_T v_A & Core_models.Option.t_Option v_T)
       Prims.l_True
@@ -116,10 +216,161 @@ let impl_10__pop
   in
   self, hax_temp_output <: (t_BinaryHeap v_T v_A & Core_models.Option.t_Option v_T)
 
+/// See [`std::collections::BinaryHeap::append`]
+let impl_10__append
+      (#v_T #v_A: Type0)
+      (#[FStar.Tactics.Typeclasses.tcresolve ()] i0: Alloc.Alloc.t_Allocator v_A)
+      (#[FStar.Tactics.Typeclasses.tcresolve ()] i1: Core_models.Cmp.t_Ord v_T)
+      (self other: t_BinaryHeap v_T v_A)
+    : Prims.Pure (t_BinaryHeap v_T v_A & t_BinaryHeap v_T v_A)
+      (requires
+        ((Rust_primitives.Hax.Int.from_machine (impl_11__len #v_T #v_A self <: usize)
+            <:
+            Hax_lib.Int.t_Int) +
+          (Rust_primitives.Hax.Int.from_machine (impl_11__len #v_T #v_A other <: usize)
+            <:
+            Hax_lib.Int.t_Int)
+          <:
+          Hax_lib.Int.t_Int) <=
+        (Rust_primitives.Hax.Int.from_machine Core_models.Num.impl_usize__MAX <: Hax_lib.Int.t_Int))
+      (fun _ -> Prims.l_True) =
+  let
+  (tmp0: Alloc.Vec.t_Vec v_T Alloc.Alloc.t_Global), (tmp1: Alloc.Vec.t_Vec v_T Alloc.Alloc.t_Global)
+  =
+    Alloc.Vec.impl_1__append #v_T #Alloc.Alloc.t_Global self._0 other._0
+  in
+  let self:t_BinaryHeap v_T v_A = { self with _0 = tmp0 } <: t_BinaryHeap v_T v_A in
+  let other:t_BinaryHeap v_T v_A = { other with _0 = tmp1 } <: t_BinaryHeap v_T v_A in
+  let _:Prims.unit = () in
+  self, other <: (t_BinaryHeap v_T v_A & t_BinaryHeap v_T v_A)
+
+/// See [`std::collections::BinaryHeap::is_empty`]
+let impl_11__is_empty
+      (#v_T #v_A: Type0)
+      (#[FStar.Tactics.Typeclasses.tcresolve ()] i0: Alloc.Alloc.t_Allocator v_A)
+      (self: t_BinaryHeap v_T v_A)
+    : bool = (Alloc.Vec.impl_1__len #v_T #Alloc.Alloc.t_Global self._0 <: usize) =. mk_usize 0
+
+/// See [`std::collections::BinaryHeap::clear`]
+let impl_11__clear
+      (#v_T #v_A: Type0)
+      (#[FStar.Tactics.Typeclasses.tcresolve ()] i0: Alloc.Alloc.t_Allocator v_A)
+      (self: t_BinaryHeap v_T v_A)
+    : t_BinaryHeap v_T v_A =
+  let self:t_BinaryHeap v_T v_A =
+    {
+      self with
+      _0
+      =
+      Alloc.Vec.from_seq #v_T
+        #Alloc.Alloc.t_Global
+        (Rust_primitives.Sequence.seq_empty #v_T () <: Rust_primitives.Sequence.t_Seq v_T)
+    }
+    <:
+    t_BinaryHeap v_T v_A
+  in
+  self
+
+/// See [`std::collections::BinaryHeap::as_slice`]: arbitrary order,
+/// which for this model is insertion order.
+let impl_11__as_slice
+      (#v_T #v_A: Type0)
+      (#[FStar.Tactics.Typeclasses.tcresolve ()] i0: Alloc.Alloc.t_Allocator v_A)
+      (self: t_BinaryHeap v_T v_A)
+    : t_Slice v_T = Alloc.Vec.impl_1__as_slice #v_T #Alloc.Alloc.t_Global self._0
+
+/// See [`std::collections::BinaryHeap::into_vec`]: arbitrary order.
+let impl_11__into_vec
+      (#v_T #v_A: Type0)
+      (#[FStar.Tactics.Typeclasses.tcresolve ()] i0: Alloc.Alloc.t_Allocator v_A)
+      (self: t_BinaryHeap v_T v_A)
+    : Alloc.Vec.t_Vec v_T Alloc.Alloc.t_Global = self._0
+
+/// See [`std::collections::BinaryHeap::iter`]: arbitrary order.
+let impl_11__iter
+      (#v_T #v_A: Type0)
+      (#[FStar.Tactics.Typeclasses.tcresolve ()] i0: Alloc.Alloc.t_Allocator v_A)
+      (self: t_BinaryHeap v_T v_A)
+    : t_Iter v_T =
+  Iter
+  (Rust_primitives.Sequence.seq_from_slice #v_T
+      (Alloc.Vec.impl_1__as_slice #v_T #Alloc.Alloc.t_Global self._0 <: t_Slice v_T))
+  <:
+  t_Iter v_T
+
+/// See [`std::collections::BinaryHeap::reserve`]: capacity is not
+/// modeled, so this leaves the contents untouched.
+let impl_11__reserve
+      (#v_T #v_A: Type0)
+      (#[FStar.Tactics.Typeclasses.tcresolve ()] i0: Alloc.Alloc.t_Allocator v_A)
+      (self: t_BinaryHeap v_T v_A)
+      (e_additional: usize)
+    : t_BinaryHeap v_T v_A = self
+
+/// See [`std::collections::BinaryHeap::reserve_exact`]
+let impl_11__reserve_exact
+      (#v_T #v_A: Type0)
+      (#[FStar.Tactics.Typeclasses.tcresolve ()] i0: Alloc.Alloc.t_Allocator v_A)
+      (self: t_BinaryHeap v_T v_A)
+      (e_additional: usize)
+    : t_BinaryHeap v_T v_A = self
+
+/// See [`std::collections::BinaryHeap::shrink_to_fit`]
+let impl_11__shrink_to_fit
+      (#v_T #v_A: Type0)
+      (#[FStar.Tactics.Typeclasses.tcresolve ()] i0: Alloc.Alloc.t_Allocator v_A)
+      (self: t_BinaryHeap v_T v_A)
+    : t_BinaryHeap v_T v_A = self
+
+/// See [`std::collections::BinaryHeap::shrink_to`]
+let impl_11__shrink_to
+      (#v_T #v_A: Type0)
+      (#[FStar.Tactics.Typeclasses.tcresolve ()] i0: Alloc.Alloc.t_Allocator v_A)
+      (self: t_BinaryHeap v_T v_A)
+      (e_min_capacity: usize)
+    : t_BinaryHeap v_T v_A = self
+
+/// See [`std::collections::BinaryHeap::try_reserve`]: the model never
+/// fails to allocate.
+let impl_11__try_reserve
+      (#v_T #v_A: Type0)
+      (#[FStar.Tactics.Typeclasses.tcresolve ()] i0: Alloc.Alloc.t_Allocator v_A)
+      (self: t_BinaryHeap v_T v_A)
+      (e_additional: usize)
+    : (t_BinaryHeap v_T v_A &
+      Core_models.Result.t_Result Prims.unit Alloc.Collections.t_TryReserveError) =
+  let hax_temp_output:Core_models.Result.t_Result Prims.unit Alloc.Collections.t_TryReserveError =
+    Core_models.Result.Result_Ok (() <: Prims.unit)
+    <:
+    Core_models.Result.t_Result Prims.unit Alloc.Collections.t_TryReserveError
+  in
+  self, hax_temp_output
+  <:
+  (t_BinaryHeap v_T v_A & Core_models.Result.t_Result Prims.unit Alloc.Collections.t_TryReserveError
+  )
+
+/// See [`std::collections::BinaryHeap::try_reserve_exact`]
+let impl_11__try_reserve_exact
+      (#v_T #v_A: Type0)
+      (#[FStar.Tactics.Typeclasses.tcresolve ()] i0: Alloc.Alloc.t_Allocator v_A)
+      (self: t_BinaryHeap v_T v_A)
+      (e_additional: usize)
+    : (t_BinaryHeap v_T v_A &
+      Core_models.Result.t_Result Prims.unit Alloc.Collections.t_TryReserveError) =
+  let hax_temp_output:Core_models.Result.t_Result Prims.unit Alloc.Collections.t_TryReserveError =
+    Core_models.Result.Result_Ok (() <: Prims.unit)
+    <:
+    Core_models.Result.t_Result Prims.unit Alloc.Collections.t_TryReserveError
+  in
+  self, hax_temp_output
+  <:
+  (t_BinaryHeap v_T v_A & Core_models.Result.t_Result Prims.unit Alloc.Collections.t_TryReserveError
+  )
+
 let impl_11__peek
       (#v_T #v_A: Type0)
-      (#[FStar.Tactics.Typeclasses.tcresolve ()] i0: Core_models.Cmp.t_Ord v_T)
-      (#[FStar.Tactics.Typeclasses.tcresolve ()] i1: Alloc.Alloc.t_Allocator v_A)
+      (#[FStar.Tactics.Typeclasses.tcresolve ()] i0: Alloc.Alloc.t_Allocator v_A)
+      (#[FStar.Tactics.Typeclasses.tcresolve ()] i1: Core_models.Cmp.t_Ord v_T)
       (self: t_BinaryHeap v_T v_A)
     : Prims.Pure (Core_models.Option.t_Option v_T)
       Prims.l_True
